Finish first sketch of foldl_evaluate (4 cheats left)

examples/cost/sumProofScript.sml
@@ -11,6 +11,8 @@ val _ = temp_delsimps ["NORMEQ_CONV"]
 
 val _ = new_theory "sumProof"
 
+val _ = ParseExtras.temp_tight_equality ()
+
 Overload monad_unitbind[local] = ``data_monad$bind``
 Overload return[local] = ``data_monad$return``
 val _ = monadsyntax.temp_add_monadsyntax()
@@ -19,6 +21,321 @@ val sum_x64_conf = (rand o rator o lhs o concl) sum_thm
 
 val _ = install_naming_overloads "sumProg";
 val _ = write_to_file sum_data_prog_def;
+
+val foldl_body = ``lookup_foldl (fromAList sum_data_prog)``
+           |> (REWRITE_CONV [sum_data_code_def] THENC EVAL)
+           |> concl |> rhs |> rand |> rand
+
+Definition foldl_body_def:
+  foldl_body = ^foldl_body
+End
+
+val Int_plus_clos_body = ``lookup_Int_+_clos (fromAList sum_data_prog)``
+           |> (REWRITE_CONV [sum_data_code_def] THENC EVAL)
+           |> concl |> rhs |> rand |> rand
+
+Definition Int_plus_clos_body_def:
+  Int_plus_clos_body = ^Int_plus_clos_body
+End
+
+val Int_plus_body = ``lookup_Int_+ (fromAList sum_data_prog)``
+           |> (REWRITE_CONV [sum_data_code_def] THENC EVAL)
+           |> concl |> rhs |> rand |> rand
+
+Definition Int_plus_body_def:
+  Int_plus_body = ^Int_plus_body
+End
+
+(* integer list of length l and with timestamps strictly bounded by tsb *)
+Definition repint_list_def:
+  (* cons *)
+  repint_list (Block ts _ [Number i; rest]) (l:num) (tsb:num) =
+     (ts < tsb ∧ l > 0 ∧ repint_list rest (l-1) tsb) ∧
+  (* nil *)
+  repint_list (Block _ tag []) (l:num) tsb = (tag = 0 ∧ l = 0) ∧
+  (* everything else *)
+  repint_list _ _ _ = F
+End
+
+Theorem repint_list_cases:
+  ∀vl n ts. repint_list vl n ts
+   ⇒ (∃ts0 tag0 i rest. vl = Block ts0 tag0 [Number i; rest] ∧ repint_list rest (n-1) ts ∧ ts0 < ts) ∨
+     (∃ts0. vl = Block ts0 0 [])
+Proof
+  ho_match_mp_tac repint_list_ind \\ rw [repint_list_def]
+QED
+
+(* The maximum amount of heap space that will be consumed by the accumulator (e) when
+   adding all number in the list
+ *)
+Definition sum_heap_size_def:
+  sum_heap_size s e []      = 0 ∧
+  sum_heap_size s e (x::xs) = MAX (space_consumed s Add [Number e; Number x])
+                                  (sum_heap_size s (e+x) xs)
+End
+
+(* The maximum amount of stack space that will be consumed by the accumulator (e) when
+   adding all number in the list
+ *)
+Definition sum_stack_size_def:
+  sum_stack_size sfs lims e []      = SOME 0 ∧
+  sum_stack_size sfs lims e (x::xs) = OPTION_MAP2 MAX (stack_consumed sfs lims (Add) [Number e; Number x])
+                                                      (sum_stack_size sfs lims (e+x) xs)
+End
+
+(* Turns a ‘v’ value into a ‘int list’; returns NONE if something goes wrong *)
+Definition repint_to_list_def:
+  repint_to_list (Block _ _ [Number i; rest]) = OPTION_MAP (CONS i) (repint_to_list rest) ∧
+  repint_to_list (Block _ 0 []) = SOME [] ∧
+  repint_to_list _ = NONE
+End
+
+(* If ‘l : v’ represents a list of integer, it is safe to turn it into
+   an actual list of integers
+*)
+Theorem repint_list_to_list_SOME:
+  ∀l n ts. repint_list l n ts ⇒ ∃il. repint_to_list l = SOME il
+Proof
+  ho_match_mp_tac repint_list_ind \\ rw [repint_to_list_def,repint_list_def]
+QED
+
+Theorem repint_list_to_list_LENGTH:
+  ∀l n ts il. repint_list l n ts ∧ repint_to_list l = SOME il ⇒ LENGTH il = n
+Proof
+  ho_match_mp_tac repint_list_ind \\ rw [repint_to_list_def,repint_list_def]
+  \\ fs [repint_to_list_def]
+QED
+
+Theorem sum_heap_size_eq:
+  ∀s1 s2 l e.
+   s1.limits = s2.limits ⇒ sum_heap_size s2 e l = sum_heap_size s1 e l
+Proof
+  ntac 2 strip_tac
+  \\ Induct \\ rw [sum_heap_size_def,space_consumed_def]
+QED
+
+Theorem Int_plus_evaluate:
+  ∀s i1 i2 sstack smax ssum.
+    (* Sizes *)
+    size_of_stack s.stack = SOME sstack ∧
+    s.locals_size = SOME 4 ∧
+    s.stack_max = SOME smax ∧
+    (* Arguments *)
+    s.locals = fromList [Number i2; Number i1] ∧
+    (* Stack frames *)
+    s.stack_frame_sizes = sum_config.word_conf.stack_frame_size ∧
+    (* Limits *)
+    stack_consumed s.stack_frame_sizes s.limits Add [Number i1; Number i2] = SOME ssum ∧
+    smax < s.limits.stack_limit ∧
+    sstack + 4 + ssum < s.limits.stack_limit ∧
+    size_of_heap s + space_consumed s Add [Number i1; Number i2] ≤ s.limits.heap_limit ∧
+    (* Code *)
+    (* Invariants *)
+    s.safe_for_space ∧
+    s.limits.arch_64_bit
+    (* s.tstamps = SOME ts ∧ *)
+    (* 1 < s.limits.length_limit *)
+    ⇒
+    ∃pkheap0.
+     evaluate (Int_plus_body,s) =
+       (SOME (Rval (Number (i1+i2))), s with <| locals := LN;
+                                                locals_size := SOME 0;
+                                                space := 0;
+                                                stack_max := SOME (MAX smax (sstack + 4 + ssum));
+                                                peak_heap_length := pkheap0
+                            |>)
+Proof
+  rw[Int_plus_body_def]
+  \\ REWRITE_TAC[to_shallow_thm,to_shallow_def]
+  \\ qpat_x_assum ‘s.locals = _’ (assume_tac o EVAL_RULE)
+  \\ qmatch_goalsub_abbrev_tac `bind _ rest_ass _`
+  \\ simp [bind_def,assign_def,cut_state_opt_def,
+           cut_state_def,cut_env_def]
+  \\ eval_goalsub_tac ``dataSem$get_vars    _ _`` \\ simp []
+  \\ simp[do_app_def,do_app_aux_def,do_space_def,
+          op_space_reset_def,set_var_def,do_stack_def]
+  \\ qunabbrev_tac ‘rest_ass’
+  \\ simp [return_def,flush_state_def,state_component_equality]
+  \\ fs [size_of_stack_def] \\ rfs []
+  (* TODO: are bignums bounded by  2 ** s.limits.length_limit *)
+  \\ conj_tac >- cheat
+  \\ conj_tac
+  >- (eval_goalsub_tac ``dataSem$state_locals_fupd _ _``
+     \\ qmatch_goalsub_abbrev_tac ‘size_of_heap ss’
+     \\ ‘ss = s’ suffices_by rw []
+     \\ UNABBREV_ALL_TAC \\ rw [state_component_equality])
+  \\ EVAL_TAC
+QED
+
+Theorem foldl_evaluate:
+  ∀n s vl il acc ts_f tag_f sstack lsize ssum smax acc ts.
+    (* Sizes *)
+    size_of_stack s.stack = SOME sstack ∧
+    s.locals_size = SOME lsize ∧
+    lookup_foldl s.stack_frame_sizes = SOME lsize ∧
+    s.stack_max = SOME smax ∧
+    s.space = 0 ∧
+    (* Arguments *)
+    s.locals = fromList [vl ; Number acc; Block ts_f tag_f [CodePtr_Int_+_clos;Number 1]] ∧
+    repint_list vl n ts ∧
+    repint_to_list vl = SOME il ∧
+    (* Stack frames *)
+    s.stack_frame_sizes = sum_config.word_conf.stack_frame_size ∧
+    sum_stack_size s.stack_frame_sizes s.limits acc il = SOME ssum ∧
+    (* Limits *)
+    smax < s.limits.stack_limit ∧
+    sstack + lsize + ssum + 4 < s.limits.stack_limit ∧
+    size_of_heap s + sum_heap_size s acc il ≤ s.limits.heap_limit ∧
+    (* Code *)
+    lookup_foldl s.code      = SOME (3,foldl_body) ∧
+    lookup_Int_+_clos s.code = SOME (3,Int_plus_clos_body) ∧
+    lookup_Int_+ s.code      = SOME (2,Int_plus_body) ∧
+    (* Invariants *)
+    s.safe_for_space ∧
+    s.limits.arch_64_bit ∧
+    s.tstamps = SOME ts ∧
+    1 < s.limits.length_limit
+    ⇒
+    ∃res lcls0 lsz0 smax0 clk0 ts0 pkheap0 stk.
+     evaluate (foldl_body,s) =
+       (SOME res, s with <| locals := lcls0;
+                            locals_size := lsz0;
+                            stack_max := SOME smax0;
+                            clock := clk0;
+                            tstamps := SOME ts0;
+                            peak_heap_length := pkheap0;
+                            stack := stk;
+                            space := 0
+                            |>) ∧
+     clk0 ≤ s.clock ∧
+     (res = (Rerr(Rabort Rtimeout_error)) ∨
+      ∃sumi. res = Rval (Number sumi) ∧ (stk = s.stack) ∧
+             smax0 = MAX smax (lsize + sstack + (if n = 0 then 0 else 4) + ssum))
+Proof
+let
+  val code_lookup   = mk_code_lookup
+                        `fromAList sum_data_prog`
+                         sum_data_code_def
+  val frame_lookup   = mk_frame_lookup
+                        `sum_config.word_conf.stack_frame_size`
+                         sum_config_def
+  val strip_assign  = mk_strip_assign code_lookup frame_lookup
+  val open_call     = mk_open_call code_lookup frame_lookup
+  val make_call     = mk_make_call open_call
+  val strip_call    = mk_strip_call open_call
+  val open_tailcall = mk_open_tailcall code_lookup frame_lookup
+  val make_tailcall = mk_make_tailcall open_tailcall
+  fun max_is t =
+    qmatch_goalsub_abbrev_tac `state_stack_max_fupd (K max0) _` >>
+    subgoal ‘max0 = SOME (^(Term t))’
+    THENL
+    [(Q.UNABBREV_TAC ‘max0’ \\ fs [small_num_def,size_of_stack_def]),
+    ASM_REWRITE_TAC [] \\ ntac 2 (pop_assum kall_tac)]
+in
+  completeInduct_on`n`
+  \\ rw[foldl_body_def,Int_plus_body_def,Int_plus_clos_body_def]
+  \\ REWRITE_TAC[to_shallow_thm,to_shallow_def]
+  \\ qpat_x_assum ‘s.locals = _’ (assume_tac o EVAL_RULE)
+  \\ drule repint_list_cases \\ reverse (rw [])
+  \\ fs [repint_list_def]
+  >- (strip_assign \\ make_if
+     \\ rw [state_component_equality]
+     \\ fs [repint_to_list_def] \\ rveq
+     \\ fs [sum_stack_size_def] \\ rveq
+     \\ fs [])
+  \\ strip_assign
+  \\ make_if
+  \\ rename1`repint_to_list (Block ts_vl tag_vl _)`
+  \\ ntac 4 strip_assign
+  \\ ONCE_REWRITE_TAC [bind_def]
+  \\ make_if
+  \\ strip_assign
+  \\ max_is ‘MAX smax (lsize + sstack)’
+  >- fs [MAX_DEF]
+  \\ strip_call
+  \\ open_tailcall
+  \\ max_is ‘MAX smax (lsize + sstack + 4)’
+  >- fs [MAX_DEF]
+  \\ qmatch_goalsub_abbrev_tac `state_safe_for_space_fupd (K safe)  _`
+  \\ ‘safe’ by
+     (qunabbrev_tac ‘safe’ \\ fs [size_of_stack_def,GREATER_DEF] \\ EVAL_TAC)
+  \\ simp [] \\ ntac 2 (pop_assum kall_tac)
+  \\ fs [repint_to_list_def] \\ rveq
+  \\ fs [sum_stack_size_def]
+  \\ qmatch_goalsub_abbrev_tac ‘bind _ _ s'’
+  \\ qspecl_then [‘s'’,‘acc’,‘i’] mp_tac Int_plus_evaluate
+  \\ disch_then (qspecl_then [‘THE (size_of_stack s'.stack)’,
+                              ‘THE (s'.stack_max)’,
+                              ‘x1’] mp_tac)
+  \\ impl_tac
+  >- (qunabbrev_tac ‘s'’ \\ rw []
+     >- fs [size_of_stack_def,size_of_stack_frame_def]
+     >- EVAL_TAC
+     >- rfs []
+     >- (Cases_on ‘x1 ≤ x2’ \\ fs [MAX_DEF,size_of_stack_frame_def,size_of_stack_def])
+     \\ fs[space_consumed_def,sum_heap_size_def]
+     \\ qmatch_goalsub_abbrev_tac ‘size_of_heap s0 + s_consumed’
+     \\ ‘size_of_heap s0 ≤ size_of_heap s’ suffices_by
+        (Cases_on ‘s_consumed ≤ sum_heap_size s (acc + i) z’ \\ fs [MAX_DEF])
+     \\ qunabbrev_tac ‘s0’
+     \\ simp [size_of_heap_def,stack_to_vs_def,toList_def,toListA_def,extract_stack_def]
+     \\ qmatch_goalsub_abbrev_tac ‘rest::rest_v’
+     (* TODO: this should be true, however one needs to move some values around to show it *)
+     \\ cheat)
+  \\ REWRITE_TAC [Int_plus_body_def,to_shallow_thm,to_shallow_def]
+  \\ rw [] \\ simp []
+  \\ qunabbrev_tac ‘s'’
+  \\ simp [pop_env_def,set_var_def]
+  \\ qunabbrev_tac ‘rest_call’
+  \\ eval_goalsub_tac ``dataSem$state_locals_fupd _ _``
+  \\ max_is ‘MAX smax (lsize + sstack + x1 + 4)’
+  >- fs [MAX_DEF]
+  \\ simp [move_def,lookup_def,set_var_def,lookup_insert]
+  \\ IF_CASES_TAC >- rw [state_component_equality]
+  \\ first_x_assum (qspec_then ‘n - 1’ mp_tac)
+  \\ simp []
+  \\ qmatch_goalsub_abbrev_tac ‘to_shallow _ s'’
+  \\ disch_then (qspecl_then [‘s'’,‘rest’,‘z’,‘ts_f’,‘tag_f’] mp_tac)
+  \\ disch_then (qspecl_then [‘THE (size_of_stack s'.stack)’,‘THE s'.locals_size’] mp_tac)
+  \\ disch_then (qspecl_then [‘x2’,‘THE s'.stack_max’,‘acc + i’,‘ts’] mp_tac)
+  \\ impl_tac
+  >- (qunabbrev_tac ‘s'’
+     \\ rw [frame_lookup,foldl_body_def,Int_plus_body_def,Int_plus_clos_body_def]
+     \\ rfs []
+     >- (Cases_on ‘x1 ≤ x2’ \\ fs [MAX_DEF])
+     >- (rfs [frame_lookup] \\ rveq \\ fs []
+         \\ Cases_on ‘x1 ≤ x2’ \\ fs [MAX_DEF])
+     >- (qmatch_goalsub_abbrev_tac ‘sum_heap_size s'’
+         \\ qspecl_then [‘s’,‘s'’,‘z’,‘acc + i’] mp_tac sum_heap_size_eq
+         \\ impl_tac >- (UNABBREV_ALL_TAC \\ rw []) \\ rw []
+         \\ fs[space_consumed_def,sum_heap_size_def]
+         \\ qmatch_asmsub_abbrev_tac ‘size_of_heap s + MAX s_consumed _’
+         \\ ‘size_of_heap s' ≤ size_of_heap s’ suffices_by
+            (Cases_on ‘s_consumed ≤ sum_heap_size s (acc + i) z’ \\ fs [MAX_DEF])
+         \\ qunabbrev_tac ‘s'’
+         \\ simp [size_of_heap_def,stack_to_vs_def,extract_stack_def]
+         \\ eval_goalsub_tac “sptree$toList _”
+         \\ eval_goalsub_tac “sptree$toList _”
+         \\ qmatch_goalsub_abbrev_tac ‘_ ++ v1 ++ v2’
+         (* TODO: again a matter of moving things around inside size_of *)
+         \\ cheat)
+     \\ fs [GREATER_DEF] \\ Cases_on ‘x1 ≤ x2’ \\ fs [MAX_DEF] \\ EVAL_TAC)
+  \\ REWRITE_TAC[to_shallow_thm,to_shallow_def,foldl_body_def]
+  \\ rw [] \\ qunabbrev_tac ‘s'’ \\ simp []
+  \\ simp [state_component_equality,GREATER_DEF] \\ fs []
+  >- (Cases_on ‘x1 ≤ x2’ \\ fs [MAX_DEF] \\ EVAL_TAC)
+  >- (reverse conj_tac
+     >- (Cases_on ‘x1 ≤ x2’ \\ fs [MAX_DEF] \\ EVAL_TAC)
+     \\ ‘n = 1’ by fs [] \\ rveq \\ fs []
+     \\ drule repint_list_cases \\ rw []
+     \\ fs [repint_list_def,repint_to_list_def]
+     \\ rveq \\ fs [sum_stack_size_def] \\ rveq
+     \\ rw [MAX_DEF])
+  >- (Cases_on ‘x1 ≤ x2’ \\ fs [MAX_DEF] \\ EVAL_TAC)
+  \\ rw [MAX_DEF]
+  \\ Cases_on ‘x1 ≤ x2’ \\ fs [MAX_DEF] \\ EVAL_TAC
+end
+QED
 
 Theorem data_safe_sum:
    ∀ffi.
@@ -108,7 +425,10 @@ in
   \\ irule data_safe_res
   \\ conj_tac >- (Cases \\ simp [] \\ IF_CASES_TAC \\ simp [])
   \\ UNABBREV_ALL_TAC
-  (* Call to sum *)
+  \\ strip_call
+  \\ ntac 4 strip_assign
+  \\ open_tailcall
+  (* TODO: plug foldl_evaluate in *)
   \\ cheat
 end
 QED
